Use Coq strings instead of idents to name external and builtin functions.
The AST.ident type represents source-level identifiers as unique positive numbers.  However, the mapping identifiers <-> AST.ident differs between runs of CompCert on different source files.  This is problematic when we need to produce or recognize external functions and builtin functions with fixed names, for example:
* in $ARCH/Machregs.v to define the register conventions for builtin functions;
* in the VST program logic from Princeton to treat thread primitives specially.

So far, we used AST.ident_of_string to recover the ident associated with a string.  However, this function is defined in OCaml and doesn't execute within Coq.  This is a problem both for VST and for future executability of CompCert within Coq.

This commit replaces "ident" by "string" in the arguments of EF_external, EF_builtin, EF_inline_asm, EF_annot, and EF_annot_val.  This provides stable names for externals and builtins, as needed.  For inline asm and annotations, it's a matter of taste, but using strings feels more natural.  EF_debug keeps using idents, since some kinds of EF_debug annotations talk about program variables.

arm/TargetPrinter.ml
@@ -777,7 +777,7 @@ module Target (Opt: PRINTER_OPTIONS) : TARGET =
           begin match ef with
           | EF_annot(txt, targs) ->
               fprintf oc "%s annotation: " comment;
-              print_annot_text preg "sp" oc (extern_atom txt) args;
+              print_annot_text preg "sp" oc (camlstring_of_coqstring txt) args;
               0
           | EF_debug(kind, txt, targs) ->
               print_debug_info comment print_file_line preg "sp" oc
@@ -785,7 +785,7 @@ module Target (Opt: PRINTER_OPTIONS) : TARGET =
               0
           | EF_inline_asm(txt, sg, clob) ->
               fprintf oc "%s begin inline assembly\n\t" comment;
-              print_inline_asm preg oc (extern_atom txt) sg args res;
+              print_inline_asm preg oc (camlstring_of_coqstring txt) sg args res;
               fprintf oc "%s end inline assembly\n" comment;
               5 (* hoping this is an upper bound...  *)
           | _ ->
