backend/CMparser.mly
@@ -35,9 +35,9 @@ type ef_token =
 let mkef sg toks =
   match toks with
   | [EFT_tok "extern"; EFT_string s] ->
-      EF_external(intern_string s, sg)
+      EF_external(coqstring_of_camlstring s, sg)
   | [EFT_tok "builtin"; EFT_string s] ->
-      EF_builtin(intern_string s, sg)
+      EF_builtin(coqstring_of_camlstring s, sg)
   | [EFT_tok "volatile"; EFT_tok "load"; EFT_chunk c] ->
       EF_vload c
   | [EFT_tok "volatile"; EFT_tok "store"; EFT_chunk c] ->
@@ -49,12 +49,12 @@ let mkef sg toks =
   | [EFT_tok "memcpy"; EFT_tok "size"; EFT_int sz; EFT_tok "align"; EFT_int al] ->
       EF_memcpy(Z.of_sint32 sz, Z.of_sint32 al)
   | [EFT_tok "annot"; EFT_string txt] ->
-      EF_annot(intern_string txt, sg.sig_args)
+      EF_annot(coqstring_of_camlstring txt, sg.sig_args)
   | [EFT_tok "annot_val"; EFT_string txt] ->
       if sg.sig_args = [] then raise Parsing.Parse_error;
-      EF_annot_val(intern_string txt, List.hd sg.sig_args)
+      EF_annot_val(coqstring_of_camlstring txt, List.hd sg.sig_args)
   | [EFT_tok "inline_asm"; EFT_string txt] ->
-      EF_inline_asm(intern_string txt, sg, [])
+      EF_inline_asm(coqstring_of_camlstring txt, sg, [])
   | _ ->
       raise Parsing.Parse_error
 
@@ -473,7 +473,7 @@ proc:
                         fn_stackspace = $8;
                         fn_body = $10 })) }
   | EXTERN STRINGLIT COLON signature 
-      { (intern_string $2, Gfun(External(EF_external(intern_string $2,$4)))) }
+      { (intern_string $2, Gfun(External(EF_external(coqstring_of_camlstring $2,$4)))) }
   | EXTERN STRINGLIT EQUAL eftoks COLON signature
       { (intern_string $2, Gfun(External(mkef $6 $4))) }
 ;
