backend/SelectLongproof.v
@@ -12,6 +12,7 @@
 
 (** Correctness of instruction selection for integer division *)
 
+Require Import String.
 Require Import Coqlib.
 Require Import AST.
 Require Import Errors.
@@ -29,81 +30,96 @@ Require Import SelectOpproof.
 Require Import SelectLong.
 
 Open Local Scope cminorsel_scope.
+Open Local Scope string_scope.
 
 (** * Axiomatization of the helper functions *)
 
-Definition external_implements (id: ident) (sg: signature) (vargs: list val) (vres: val) : Prop :=
+Definition external_implements (name: string) (sg: signature) (vargs: list val) (vres: val) : Prop :=
   forall F V (ge: Genv.t F V) m,
-  external_call (EF_external id sg) ge vargs m E0 vres m.
+  external_call (EF_external name sg) ge vargs m E0 vres m.
 
-Definition builtin_implements (id: ident) (sg: signature) (vargs: list val) (vres: val) : Prop :=
+Definition builtin_implements (name: string) (sg: signature) (vargs: list val) (vres: val) : Prop :=
   forall F V (ge: Genv.t F V) m,
-  external_call (EF_builtin id sg) ge vargs m E0 vres m.
+  external_call (EF_builtin name sg) ge vargs m E0 vres m.
 
 Axiom i64_helpers_correct :
-    (forall x z, Val.longoffloat x = Some z -> external_implements i64_dtos sig_f_l (x::nil) z)
- /\ (forall x z, Val.longuoffloat x = Some z -> external_implements i64_dtou sig_f_l (x::nil) z)
- /\ (forall x z, Val.floatoflong x = Some z -> external_implements i64_stod sig_l_f (x::nil) z)
- /\ (forall x z, Val.floatoflongu x = Some z -> external_implements i64_utod sig_l_f (x::nil) z)
- /\ (forall x z, Val.singleoflong x = Some z -> external_implements i64_stof sig_l_s (x::nil) z)
- /\ (forall x z, Val.singleoflongu x = Some z -> external_implements i64_utof sig_l_s (x::nil) z)
- /\ (forall x, builtin_implements i64_neg sig_l_l (x::nil) (Val.negl x))
- /\ (forall x y, builtin_implements i64_add sig_ll_l (x::y::nil) (Val.addl x y))
- /\ (forall x y, builtin_implements i64_sub sig_ll_l (x::y::nil) (Val.subl x y))
- /\ (forall x y, builtin_implements i64_mul sig_ii_l (x::y::nil) (Val.mull' x y))
- /\ (forall x y z, Val.divls x y = Some z -> external_implements i64_sdiv sig_ll_l (x::y::nil) z)
- /\ (forall x y z, Val.divlu x y = Some z -> external_implements i64_udiv sig_ll_l (x::y::nil) z)
- /\ (forall x y z, Val.modls x y = Some z -> external_implements i64_smod sig_ll_l (x::y::nil) z)
- /\ (forall x y z, Val.modlu x y = Some z -> external_implements i64_umod sig_ll_l (x::y::nil) z)
- /\ (forall x y, external_implements i64_shl sig_li_l (x::y::nil) (Val.shll x y))
- /\ (forall x y, external_implements i64_shr sig_li_l (x::y::nil) (Val.shrlu x y))
- /\ (forall x y, external_implements i64_sar sig_li_l (x::y::nil) (Val.shrl x y)).
+    (forall x z, Val.longoffloat x = Some z -> external_implements "__i64_dtos" sig_f_l (x::nil) z)
+ /\ (forall x z, Val.longuoffloat x = Some z -> external_implements "__i64_dtou" sig_f_l (x::nil) z)
+ /\ (forall x z, Val.floatoflong x = Some z -> external_implements "__i64_stod" sig_l_f (x::nil) z)
+ /\ (forall x z, Val.floatoflongu x = Some z -> external_implements "__i64_utod" sig_l_f (x::nil) z)
+ /\ (forall x z, Val.singleoflong x = Some z -> external_implements "__i64_stof" sig_l_s (x::nil) z)
+ /\ (forall x z, Val.singleoflongu x = Some z -> external_implements "__i64_utof" sig_l_s (x::nil) z)
+ /\ (forall x, builtin_implements "__builtin_negl" sig_l_l (x::nil) (Val.negl x))
+ /\ (forall x y, builtin_implements "__builtin_addl" sig_ll_l (x::y::nil) (Val.addl x y))
+ /\ (forall x y, builtin_implements "__builtin_subl" sig_ll_l (x::y::nil) (Val.subl x y))
+ /\ (forall x y, builtin_implements "__builtin_mull" sig_ii_l (x::y::nil) (Val.mull' x y))
+ /\ (forall x y z, Val.divls x y = Some z -> external_implements "__i64_sdiv" sig_ll_l (x::y::nil) z)
+ /\ (forall x y z, Val.divlu x y = Some z -> external_implements "__i64_udiv" sig_ll_l (x::y::nil) z)
+ /\ (forall x y z, Val.modls x y = Some z -> external_implements "__i64_smod" sig_ll_l (x::y::nil) z)
+ /\ (forall x y z, Val.modlu x y = Some z -> external_implements "__i64_umod" sig_ll_l (x::y::nil) z)
+ /\ (forall x y, external_implements "__i64_shl" sig_li_l (x::y::nil) (Val.shll x y))
+ /\ (forall x y, external_implements "__i64_shr" sig_li_l (x::y::nil) (Val.shrlu x y))
+ /\ (forall x y, external_implements "__i64_sar" sig_li_l (x::y::nil) (Val.shrl x y)).
 
-Definition helper_declared {F V: Type} (ge: Genv.t (AST.fundef F) V) (name: ident) (sg: signature) : Prop :=
-  exists b, Genv.find_symbol ge name = Some b
+Definition helper_declared {F V: Type} (ge: Genv.t (AST.fundef F) V) (id: ident) (name: string) (sg: signature) : Prop :=
+  exists b, Genv.find_symbol ge id = Some b
          /\ Genv.find_funct_ptr ge b = Some (External (EF_external name sg)).
+
+Definition helper_functions_declared {F V: Type} (ge: Genv.t (AST.fundef F) V) (hf: helper_functions) : Prop :=
+     helper_declared ge hf.(i64_dtos) "__i64_dtos" sig_f_l
+  /\ helper_declared ge hf.(i64_dtou) "__i64_dtou" sig_f_l
+  /\ helper_declared ge hf.(i64_stod) "__i64_stod" sig_l_f
+  /\ helper_declared ge hf.(i64_utod) "__i64_utod" sig_l_f
+  /\ helper_declared ge hf.(i64_stof) "__i64_stof" sig_l_s
+  /\ helper_declared ge hf.(i64_utof) "__i64_utof" sig_l_s
+  /\ helper_declared ge hf.(i64_sdiv) "__i64_sdiv" sig_ll_l
+  /\ helper_declared ge hf.(i64_udiv) "__i64_udiv" sig_ll_l
+  /\ helper_declared ge hf.(i64_smod) "__i64_smod" sig_ll_l
+  /\ helper_declared ge hf.(i64_umod) "__i64_umod" sig_ll_l
+  /\ helper_declared ge hf.(i64_shl) "__i64_shl" sig_li_l
+  /\ helper_declared ge hf.(i64_shr) "__i64_shr" sig_li_l
+  /\ helper_declared ge hf.(i64_sar) "__i64_sar" sig_li_l.
 
 (** * Correctness of the instruction selection functions for 64-bit operators *)
 
 Section CMCONSTR.
 
 Variable ge: genv.
-Hypothesis HELPERS:
-  forall name sg, In (name, sg) i64_helpers -> helper_declared ge name sg.
+Variable hf: helper_functions.
+Hypothesis HELPERS: helper_functions_declared ge hf.
 Variable sp: val.
 Variable e: env.
 Variable m: mem.
 
-Ltac UseHelper :=
-  generalize i64_helpers_correct; intros;
-  repeat (eauto; match goal with | [ H: _ /\ _ |- _ ] => destruct H end).
+Ltac UseHelper := decompose [Logic.and] i64_helpers_correct; eauto.
+Ltac DeclHelper := red in HELPERS; decompose [Logic.and] HELPERS; eauto.
 
 Lemma eval_helper:
-  forall le id sg args vargs vres,
+  forall le id name sg args vargs vres,
   eval_exprlist ge sp e m le args vargs ->
-  In (id, sg) i64_helpers ->
-  external_implements id sg vargs vres ->
+  helper_declared ge id name sg  ->
+  external_implements name sg vargs vres ->
   eval_expr ge sp e m le (Eexternal id sg args) vres.
 Proof.
-  intros. exploit HELPERS; eauto. intros (b & A & B). econstructor; eauto.
+  intros. destruct H0 as (b & P & Q). econstructor; eauto.
 Qed.
 
 Corollary eval_helper_1:
-  forall le id sg arg1 varg1 vres,
+  forall le id name sg arg1 varg1 vres,
   eval_expr ge sp e m le arg1 varg1 ->
-  In (id, sg) i64_helpers ->
-  external_implements id sg (varg1::nil) vres ->
+  helper_declared ge id name sg  ->
+  external_implements name sg (varg1::nil) vres ->
   eval_expr ge sp e m le (Eexternal id sg (arg1 ::: Enil)) vres.
 Proof.
   intros. eapply eval_helper; eauto. constructor; auto. constructor.
 Qed.
 
 Corollary eval_helper_2:
-  forall le id sg arg1 arg2 varg1 varg2 vres,
+  forall le id name sg arg1 arg2 varg1 varg2 vres,
   eval_expr ge sp e m le arg1 varg1 ->
   eval_expr ge sp e m le arg2 varg2 ->
-  In (id, sg) i64_helpers ->
-  external_implements id sg (varg1::varg2::nil) vres ->
+  helper_declared ge id name sg  ->
+  external_implements name sg (varg1::varg2::nil) vres ->
   eval_expr ge sp e m le (Eexternal id sg (arg1 ::: arg2 ::: Enil)) vres.
 Proof.
   intros. eapply eval_helper; eauto. constructor; auto. constructor; auto. constructor.
@@ -394,51 +410,47 @@ Theorem eval_longoffloat:
   forall le a x y,
   eval_expr ge sp e m le a x ->
   Val.longoffloat x = Some y ->
-  exists v, eval_expr ge sp e m le (longoffloat a) v /\ Val.lessdef y v.
+  exists v, eval_expr ge sp e m le (longoffloat hf a) v /\ Val.lessdef y v.
 Proof.
   intros; unfold longoffloat. econstructor; split. 
-  eapply eval_helper_1; eauto. simpl; auto. UseHelper.
-  auto.
+  eapply eval_helper_1; eauto. DeclHelper. UseHelper. auto.
 Qed.
 
 Theorem eval_longuoffloat:
   forall le a x y,
   eval_expr ge sp e m le a x ->
   Val.longuoffloat x = Some y ->
-  exists v, eval_expr ge sp e m le (longuoffloat a) v /\ Val.lessdef y v.
+  exists v, eval_expr ge sp e m le (longuoffloat hf a) v /\ Val.lessdef y v.
 Proof.
   intros; unfold longuoffloat. econstructor; split. 
-  eapply eval_helper_1; eauto. simpl; auto. UseHelper. 
-  auto.
+  eapply eval_helper_1; eauto. DeclHelper. UseHelper. auto.
 Qed.
 
 Theorem eval_floatoflong:
   forall le a x y,
   eval_expr ge sp e m le a x ->
   Val.floatoflong x = Some y ->
-  exists v, eval_expr ge sp e m le (floatoflong a) v /\ Val.lessdef y v.
+  exists v, eval_expr ge sp e m le (floatoflong hf a) v /\ Val.lessdef y v.
 Proof.
   intros; unfold floatoflong. econstructor; split. 
-  eapply eval_helper_1; eauto. simpl; auto. UseHelper. 
-  auto.
+  eapply eval_helper_1; eauto. DeclHelper. UseHelper. auto.
 Qed.
 
 Theorem eval_floatoflongu:
   forall le a x y,
   eval_expr ge sp e m le a x ->
   Val.floatoflongu x = Some y ->
-  exists v, eval_expr ge sp e m le (floatoflongu a) v /\ Val.lessdef y v.
+  exists v, eval_expr ge sp e m le (floatoflongu hf a) v /\ Val.lessdef y v.
 Proof.
   intros; unfold floatoflongu. econstructor; split. 
-  eapply eval_helper_1; eauto. simpl; auto. UseHelper. 
-  auto.
+  eapply eval_helper_1; eauto. DeclHelper. UseHelper. auto.
 Qed.
 
 Theorem eval_longofsingle:
   forall le a x y,
   eval_expr ge sp e m le a x ->
   Val.longofsingle x = Some y ->
-  exists v, eval_expr ge sp e m le (longofsingle a) v /\ Val.lessdef y v.
+  exists v, eval_expr ge sp e m le (longofsingle hf a) v /\ Val.lessdef y v.
 Proof.
   intros; unfold longofsingle.
   destruct x; simpl in H0; inv H0. destruct (Float32.to_long f) as [n|] eqn:EQ; simpl in H2; inv H2.
@@ -452,7 +464,7 @@ Theorem eval_longuofsingle:
   forall le a x y,
   eval_expr ge sp e m le a x ->
   Val.longuofsingle x = Some y ->
-  exists v, eval_expr ge sp e m le (longuofsingle a) v /\ Val.lessdef y v.
+  exists v, eval_expr ge sp e m le (longuofsingle hf a) v /\ Val.lessdef y v.
 Proof.
   intros; unfold longuofsingle.
   destruct x; simpl in H0; inv H0. destruct (Float32.to_longu f) as [n|] eqn:EQ; simpl in H2; inv H2.
@@ -466,22 +478,20 @@ Theorem eval_singleoflong:
   forall le a x y,
   eval_expr ge sp e m le a x ->
   Val.singleoflong x = Some y ->
-  exists v, eval_expr ge sp e m le (singleoflong a) v /\ Val.lessdef y v.
+  exists v, eval_expr ge sp e m le (singleoflong hf a) v /\ Val.lessdef y v.
 Proof.
   intros; unfold singleoflong. econstructor; split. 
-  eapply eval_helper_1; eauto. simpl; auto 20. UseHelper. 
-  auto.
+  eapply eval_helper_1; eauto. DeclHelper. UseHelper. auto.
 Qed.
 
 Theorem eval_singleoflongu:
   forall le a x y,
   eval_expr ge sp e m le a x ->
   Val.singleoflongu x = Some y ->
-  exists v, eval_expr ge sp e m le (singleoflongu a) v /\ Val.lessdef y v.
+  exists v, eval_expr ge sp e m le (singleoflongu hf a) v /\ Val.lessdef y v.
 Proof.
   intros; unfold singleoflongu. econstructor; split. 
-  eapply eval_helper_1; eauto. simpl; auto 20. UseHelper. 
-  auto.
+  eapply eval_helper_1; eauto. DeclHelper. UseHelper. auto.
 Qed.
 
 Theorem eval_andl: binary_constructor_sound andl Val.andl.
@@ -578,7 +588,7 @@ Qed.
 
 Lemma eval_shllimm:
   forall n,
-  unary_constructor_sound (fun e => shllimm e n) (fun v => Val.shll v (Vint n)).
+  unary_constructor_sound (fun e => shllimm hf e n) (fun v => Val.shll v (Vint n)).
 Proof.
   unfold shllimm; red; intros.
   apply eval_shift_imm; intros.
@@ -608,11 +618,10 @@ Proof.
     simpl. erewrite <- Int64.decompose_shl_2. instantiate (1 := Int64.hiword i). 
     rewrite Int64.ofwords_recompose. auto. auto.
   + (* n >= 64 *)
-    econstructor; split. eapply eval_helper_2; eauto. EvalOp. 
-    simpl; auto 20. UseHelper. auto.
+    econstructor; split. eapply eval_helper_2; eauto. EvalOp. DeclHelper. UseHelper. auto.
 Qed.
 
-Theorem eval_shll: binary_constructor_sound shll Val.shll.
+Theorem eval_shll: binary_constructor_sound (shll hf) Val.shll.
 Proof.
   unfold shll; red; intros.
   destruct (is_intconst b) as [n|] eqn:IC.
@@ -620,12 +629,12 @@ Proof.
   exploit is_intconst_sound; eauto. intros EQ; subst y; clear H0.
   eapply eval_shllimm; eauto.
 - (* General case *)
-  econstructor; split. eapply eval_helper_2; eauto. simpl; auto 20. UseHelper. auto.
+  econstructor; split. eapply eval_helper_2; eauto. DeclHelper. UseHelper. auto.
 Qed.
 
 Lemma eval_shrluimm:
   forall n,
-  unary_constructor_sound (fun e => shrluimm e n) (fun v => Val.shrlu v (Vint n)).
+  unary_constructor_sound (fun e => shrluimm hf e n) (fun v => Val.shrlu v (Vint n)).
 Proof.
   unfold shrluimm; red; intros. apply eval_shift_imm; intros.
   + (* n = 0 *)
@@ -654,10 +663,10 @@ Proof.
     simpl. erewrite <- Int64.decompose_shru_2. instantiate (1 := Int64.loword i). 
     rewrite Int64.ofwords_recompose. auto. auto.
   + (* n >= 64 *)
-    econstructor; split. eapply eval_helper_2; eauto. EvalOp. simpl; auto 20. UseHelper. auto.
+    econstructor; split. eapply eval_helper_2; eauto. EvalOp. DeclHelper. UseHelper. auto.
 Qed.
 
-Theorem eval_shrlu: binary_constructor_sound shrlu Val.shrlu.
+Theorem eval_shrlu: binary_constructor_sound (shrlu hf) Val.shrlu.
 Proof.
   unfold shrlu; red; intros.
   destruct (is_intconst b) as [n|] eqn:IC.
@@ -665,12 +674,12 @@ Proof.
   exploit is_intconst_sound; eauto. intros EQ; subst y; clear H0.
   eapply eval_shrluimm; eauto.
 - (* General case *)
-  econstructor; split. eapply eval_helper_2; eauto. simpl; auto 20. UseHelper. auto.
+  econstructor; split. eapply eval_helper_2; eauto. DeclHelper. UseHelper. auto.
 Qed.
 
 Lemma eval_shrlimm:
   forall n,
-  unary_constructor_sound (fun e => shrlimm e n) (fun v => Val.shrl v (Vint n)).
+  unary_constructor_sound (fun e => shrlimm hf e n) (fun v => Val.shrl v (Vint n)).
 Proof.
   unfold shrlimm; red; intros. apply eval_shift_imm; intros.
   + (* n = 0 *)
@@ -703,10 +712,10 @@ Proof.
     erewrite <- Int64.decompose_shr_2. instantiate (1 := Int64.loword i). 
     rewrite Int64.ofwords_recompose. auto. auto.
   + (* n >= 64 *)
-    econstructor; split. eapply eval_helper_2; eauto. EvalOp. simpl; auto 20. UseHelper. auto.
+    econstructor; split. eapply eval_helper_2; eauto. EvalOp. DeclHelper. UseHelper. auto.
 Qed.
 
-Theorem eval_shrl: binary_constructor_sound shrl Val.shrl.
+Theorem eval_shrl: binary_constructor_sound (shrl hf) Val.shrl.
 Proof.
   unfold shrl; red; intros.
   destruct (is_intconst b) as [n|] eqn:IC.
@@ -714,17 +723,17 @@ Proof.
   exploit is_intconst_sound; eauto. intros EQ; subst y; clear H0.
   eapply eval_shrlimm; eauto.
 - (* General case *)
-  econstructor; split. eapply eval_helper_2; eauto. simpl; auto 20. UseHelper. auto.
+  econstructor; split. eapply eval_helper_2; eauto. DeclHelper. UseHelper. auto.
 Qed.
 
 Theorem eval_addl: binary_constructor_sound addl Val.addl.
 Proof.
   unfold addl; red; intros.
-  set (default := Ebuiltin (EF_builtin i64_add sig_ll_l) (a ::: b ::: Enil)).
+  set (default := Ebuiltin (EF_builtin "__builtin_addl" sig_ll_l) (a ::: b ::: Enil)).
   assert (DEFAULT:
     exists v, eval_expr ge sp e m le default v /\ Val.lessdef (Val.addl x y) v).
   {
-    econstructor; split. eapply eval_builtin_2; eauto. simpl; auto 20. UseHelper. auto. 
+    econstructor; split. eapply eval_builtin_2; eauto. UseHelper. auto. 
   }
   destruct (is_longconst a) as [p|] eqn:LC1;
   destruct (is_longconst b) as [q|] eqn:LC2.
@@ -743,11 +752,11 @@ Qed.
 Theorem eval_subl: binary_constructor_sound subl Val.subl.
 Proof.
   unfold subl; red; intros.
-  set (default := Ebuiltin (EF_builtin i64_sub sig_ll_l) (a ::: b ::: Enil)).
+  set (default := Ebuiltin (EF_builtin "__builtin_subl" sig_ll_l) (a ::: b ::: Enil)).
   assert (DEFAULT:
     exists v, eval_expr ge sp e m le default v /\ Val.lessdef (Val.subl x y) v).
   {
-    econstructor; split. eapply eval_builtin_2; eauto. simpl; auto 20. UseHelper. auto. 
+    econstructor; split. eapply eval_builtin_2; eauto. UseHelper. auto. 
   }
   destruct (is_longconst a) as [p|] eqn:LC1;
   destruct (is_longconst b) as [q|] eqn:LC2.
@@ -778,7 +787,7 @@ Proof.
   exploit eval_add. eexact E2. eexact E3. intros [v5 [E5 L5]].
   exploit eval_add. eexact E5. eexact E4. intros [v6 [E6 L6]].
   exists (Val.longofwords v6 (Val.loword p)); split.
-  EvalOp. eapply eval_builtin_2; eauto. simpl; auto 20. UseHelper. 
+  EvalOp. eapply eval_builtin_2; eauto. UseHelper. 
   intros. unfold le1, p in *; subst; simpl in *.
   inv L3. inv L4. inv L5. simpl in L6. inv L6. 
   simpl. f_equal. symmetry. apply Int64.decompose_mul. 
@@ -786,7 +795,7 @@ Proof.
 Qed.
 
 Lemma eval_mullimm:
-  forall n, unary_constructor_sound (fun a => mullimm a n) (fun v => Val.mull v (Vlong n)).
+  forall n, unary_constructor_sound (fun a => mullimm hf a n) (fun v => Val.mull v (Vlong n)).
 Proof.
   unfold mullimm; red; intros.
   predSpec Int64.eq Int64.eq_spec n Int64.zero.
@@ -816,7 +825,7 @@ Proof.
   apply eval_mull_base; auto. apply eval_longconst. 
 Qed.
 
-Theorem eval_mull: binary_constructor_sound mull Val.mull.
+Theorem eval_mull: binary_constructor_sound (mull hf) Val.mull.
 Proof.
   unfold mull; red; intros.
   destruct (is_longconst a) as [p|] eqn:LC1;
@@ -834,10 +843,10 @@ Proof.
 Qed.
 
 Lemma eval_binop_long:
-  forall id sem le a b x y z,
+  forall id name sem le a b x y z,
   (forall p q, x = Vlong p -> y = Vlong q -> z = Vlong (sem p q)) ->
-  external_implements id sig_ll_l (x::y::nil) z ->
-  In (id, sig_ll_l) i64_helpers ->
+  helper_declared ge id name sig_ll_l ->
+  external_implements name sig_ll_l (x::y::nil) z ->
   eval_expr ge sp e m le a x ->
   eval_expr ge sp e m le b y ->
   exists v, eval_expr ge sp e m le (binop_long id sem a b) v /\ Val.lessdef z v.
@@ -857,15 +866,14 @@ Theorem eval_divl:
   eval_expr ge sp e m le a x ->
   eval_expr ge sp e m le b y ->
   Val.divls x y = Some z ->
-  exists v, eval_expr ge sp e m le (divl a b) v /\ Val.lessdef z v.
+  exists v, eval_expr ge sp e m le (divl hf a b) v /\ Val.lessdef z v.
 Proof.
   intros. eapply eval_binop_long; eauto. 
   intros; subst; simpl in H1.
   destruct (Int64.eq q Int64.zero
          || Int64.eq p (Int64.repr Int64.min_signed) && Int64.eq q Int64.mone); inv H1. 
   auto.
-  UseHelper. 
-  simpl; auto 20.
+  DeclHelper. UseHelper. 
 Qed.
 
 Theorem eval_modl:
@@ -873,15 +881,14 @@ Theorem eval_modl:
   eval_expr ge sp e m le a x ->
   eval_expr ge sp e m le b y ->
   Val.modls x y = Some z ->
-  exists v, eval_expr ge sp e m le (modl a b) v /\ Val.lessdef z v.
+  exists v, eval_expr ge sp e m le (modl hf a b) v /\ Val.lessdef z v.
 Proof.
   intros. eapply eval_binop_long; eauto. 
   intros; subst; simpl in H1.
   destruct (Int64.eq q Int64.zero
          || Int64.eq p (Int64.repr Int64.min_signed) && Int64.eq q Int64.mone); inv H1. 
   auto.
-  UseHelper. 
-  simpl; auto 20.
+  DeclHelper. UseHelper.
 Qed.
 
 Theorem eval_divlu:
@@ -889,14 +896,14 @@ Theorem eval_divlu:
   eval_expr ge sp e m le a x ->
   eval_expr ge sp e m le b y ->
   Val.divlu x y = Some z ->
-  exists v, eval_expr ge sp e m le (divlu a b) v /\ Val.lessdef z v.
+  exists v, eval_expr ge sp e m le (divlu hf a b) v /\ Val.lessdef z v.
 Proof.
   intros. unfold divlu. 
-  set (default := Eexternal i64_udiv sig_ll_l (a ::: b ::: Enil)).
+  set (default := Eexternal hf.(i64_udiv) sig_ll_l (a ::: b ::: Enil)).
   assert (DEFAULT:
     exists v, eval_expr ge sp e m le default v /\ Val.lessdef z v).
   {
-    econstructor; split. eapply eval_helper_2; eauto. simpl; auto 20. UseHelper. auto. 
+    econstructor; split. eapply eval_helper_2; eauto. DeclHelper. UseHelper. auto. 
   }
   destruct (is_longconst a) as [p|] eqn:LC1;
   destruct (is_longconst b) as [q|] eqn:LC2.
@@ -932,14 +939,14 @@ Theorem eval_modlu:
   eval_expr ge sp e m le a x ->
   eval_expr ge sp e m le b y ->
   Val.modlu x y = Some z ->
-  exists v, eval_expr ge sp e m le (modlu a b) v /\ Val.lessdef z v.
+  exists v, eval_expr ge sp e m le (modlu hf a b) v /\ Val.lessdef z v.
 Proof.
   intros. unfold modlu. 
-  set (default := Eexternal i64_umod sig_ll_l (a ::: b ::: Enil)).
+  set (default := Eexternal hf.(i64_umod) sig_ll_l (a ::: b ::: Enil)).
   assert (DEFAULT:
     exists v, eval_expr ge sp e m le default v /\ Val.lessdef z v).
   {
-    econstructor; split. eapply eval_helper_2; eauto. simpl; auto 20. UseHelper. auto. 
+    econstructor; split. eapply eval_helper_2; eauto. DeclHelper. UseHelper. auto. 
   }
   destruct (is_longconst a) as [p|] eqn:LC1;
   destruct (is_longconst b) as [q|] eqn:LC2.
